\documentclass[12pt, a4paper, oneside]{ctexart}
\usepackage{amsmath, amsthm, amssymb, bm, color, framed, graphicx, hyperref, mathrsfs}
\usepackage{geometry}
\geometry{left=2.54cm,right=2.54cm,top=3.18cm,bottom=3.18cm}
\title{\textbf{数理逻辑作业: lianxi4}}
\author{hsuchou}
\date{\today}
\linespread{1.4}
\definecolor{shadecolor}{RGB}{240,249,254}
\newcounter{problemname}
\newenvironment{problem}{\begin{shaded}\stepcounter{problemname}\par\noindent\textbf{题目\arabic{problemname}. }}{\end{shaded}\par}
\newenvironment{solution}{\par\noindent\textbf{解答. }}{\par}
\newenvironment{note}{\par\noindent\textbf{题目\arabic{problemname}的注记. }}{\par}
\newcounter{lemmaname}
\newenvironment{lemma}{\stepcounter{lemmaname}\par\noindent\textbf{引理\arabic{lemmaname}. }}{\par}

\begin{document}
\maketitle

\subsection*{0. 引理}
\begin{lemma}
(逆否) 
\begin{align*}
    \text{if }A\vdash B,\text{ then } \neg B\vdash \neg A.
\end{align*}
\begin{proof}
    \begin{align*}
        \neg B, A&\vdash \neg B &(\in)\\
        A&\vdash B &(\text{assumption})\\
        \neg B, A &\vdash B &(+)\\
        \neg B&\vdash \neg A &(\neg^-)
    \end{align*}
\end{proof}
\end{lemma}
\begin{lemma}
\begin{align*}
    \neg(A\rightarrow B)\vdash A\land \neg B.
\end{align*}
\begin{proof}
    \begin{align*}
        \neg A, A, \neg B&\vdash A&(\in)\\
        \neg A, A, \neg B&\vdash\neg A&(\in)\\
        \neg A, A&\vdash B&(\neg^-)\\
        \neg A&\vdash A\rightarrow B&(\rightarrow^+)\\
        B, A&\vdash B&(\in)\\
        B&\vdash A\rightarrow B&(\rightarrow^+)\\
        \neg(A\rightarrow B)&\vdash\neg B &(\text{逆否})\\
        \neg(A\rightarrow B)&\vdash A &(\text{逆否})\\
        \neg(A\rightarrow B)&\vdash A\land\neg B &(\land^+)
    \end{align*}
\end{proof}
\end{lemma}
\begin{lemma}
($\neg\neg^-$)
\begin{align*}
    \neg\neg A\vdash A
\end{align*}
\begin{proof}
    \begin{align*}
        \neg\neg A,\neg A&\vdash\neg A&(\in)\\
        \neg\neg A,\neg A&\vdash\neg\neg A&(\in)\\
        \neg\neg A&\vdash A&(\neg^-)
    \end{align*}
\end{proof}

\end{lemma}

\subsection*{1. Using the natural deduction rules to prove the following statements}
\begin{problem}
\begin{equation*}
    \neg\exists x A(x)
    \vdash\dashv
    \forall x \neg A(x).
\end{equation*}
\end{problem}
\begin{solution}
    先证 $\vdash$：
    \begin{align*}
        A(u)&\vdash A(u) &(\text{ref})\\
        A(u)&\vdash \exists x A(x)  &(\exists^+, x\text{不在}A(u)\text{中出现})\\
        \neg \exists x A(x)&\vdash \neg A(u) &(\text{逆否}) \\
        \neg\exists x A(x)&\vdash\forall x \neg A(x)
        &(\forall^+,x\text{不在}A(u)\text{中自由出现})
    \end{align*}
    后证 $\dashv$：
    \begin{align*}
        \forall x\neg A(x)&\vdash\forall x \neg A(x)&(\text{ref})\\
        \forall x\neg A(x)&\vdash \neg A(u) &(\forall^-)\\
        A(u)&\vdash \neg \forall x\neg A(x)&(\text{逆否})\\
        \exists xA(x)&\vdash\neg \forall x\neg A(x)
        &(\exists^-,u\text{不在}\neg\forall x\neg A(x)\text{出现})\\
        \forall x \neg A(x), \exists xA(x)&\vdash
        \neg \forall x\neg A(x)&(+)\\
        \forall x \neg A(x), \exists xA(x)&\vdash
        \forall x \neg A(x)&(\in)\\
        \forall x \neg A(x)&\vdash \neg\exists x A(x)&(\neg^-)
    \end{align*}
    综上，该statement成立。
\end{solution}
\begin{problem}
\begin{equation*}
    \exists xA(x)\rightarrow B
    \vdash\dashv
    \forall x(A(x)\rightarrow B),
\end{equation*}
where $x$ does not occur in $B$.
\end{problem}
\begin{solution}
    先证 $\vdash$：
    \begin{align*}
        \exists xA(x)\rightarrow B, A(u)
        &\vdash A(u)
        &(\in)\\
        \exists xA(x)\rightarrow B, A(u)
        &\vdash \exists xA(x)
        &(\exists^+)\\
        \exists xA(x)\rightarrow B, A(u)
        &\vdash \exists xA(x)\rightarrow B
        &(\in)\\
        \exists xA(x)\rightarrow B, A(u)
        &\vdash B
        &(\rightarrow^-)\\
        \exists xA(x)\rightarrow B 
        &\vdash A(u)\rightarrow B
        &(\rightarrow^+)\\
        \exists xA(x)\rightarrow B 
        &\vdash \forall x(A(x)\rightarrow B)
        &(\forall^+, u\text{不在}\exists xA(x)\rightarrow B\text{中出现})
    \end{align*}
    后证 $\dashv$：
    \begin{align*}
        \forall x(A(x)\rightarrow B)&\vdash
        \forall x(A(x)\rightarrow B)&(\text{ref})\\
        \forall x(A(x)\rightarrow B)
        &\vdash A(u)\rightarrow B &(\forall^-)\\
        \forall x(A(x)\rightarrow B), A(u)
        &\vdash A(u)\rightarrow B &(+)\\
        \forall x(A(x)\rightarrow B), A(u)
        &\vdash A(u) &(\in)\\
        \forall x(A(x)\rightarrow B), A(u)
        &\vdash B &(\rightarrow^-)\\
        \forall x(A(x)\rightarrow B), \exists xA(x)
        &\vdash B 
        &(\exists^-,u\text{不在}\forall x(A(x)\rightarrow B), B\text{中出现})\\
        \forall x(A(x)\rightarrow B)
        &\vdash \exists xA(x)\rightarrow B &(\rightarrow^+)
    \end{align*}
\end{solution}
\subsection*{2.  Prove the following statements}
\begin{problem}
\begin{equation*}
    \vdash
    \forall x\forall y r(x,y)
    \rightarrow
    \forall x r(x,x),
\end{equation*}
where $r$ is a binary predicate symbol.
\end{problem}
\begin{solution}
    \begin{align*}
        \forall x\forall y r(x,y)
        &\vdash
        \forall x\forall y r(x,y) &(\text{ref})
        \\
        \forall x\forall y r(x,y)
        &\vdash
        \forall yr(u,y) &(\forall^-)
        \\
        \forall yr(u,y)
        &\vdash
        r(u,u) &(\forall^-)
        \\
        \forall yr(u,y)
        &\vdash
        \forall x r(x,x), &(\forall^+)
        \\
        \forall x\forall y r(x,y)&\vdash
        \forall x r(x,x), &(\text{trans})
        \\
        &\vdash
        \forall x\forall y r(x,y)
        \rightarrow
        \forall x r(x,x), &(\rightarrow^+)
    \end{align*}
\end{solution}
\begin{problem}
\begin{equation*}
    \vdash
    \forall x A(x)\rightarrow
    \forall x(A(x)\lor B(x))
\end{equation*}
\end{problem}
\begin{solution}
    \begin{align*}
        \forall x A(x)&\vdash
        \forall xA(x)&(\text{ref})\\
        \forall x A(x)&\vdash
        A(u)&(\forall^-)\\
        \forall x A(x)&\vdash
        A(u)\lor B(u)&(\lor^+)\\
        \forall x A(x)&\vdash
        \forall x(A(x)\lor B(x))&(\forall^+)\\
        &\vdash
        \forall x A(x)\rightarrow
        \forall x(A(x)\lor B(x))&(\rightarrow^+)
    \end{align*}
\end{solution}

\begin{problem}
\begin{equation*}
    \vdash
    (\exists xA(x)\rightarrow\forall x B(x))
    \rightarrow
    \forall x(A(x)\rightarrow B(x))
\end{equation*}
\end{problem}
\begin{solution}
    \begin{align*}
        \exists xA(x)\rightarrow\forall x B(x), A(u)
        &\vdash
        A(u) &(\text{ref})\\
        \exists xA(x)\rightarrow\forall x B(x), A(u)
        &\vdash
        \exists xA(x) &(\exists^+)\\
        \exists xA(x)\rightarrow\forall x B(x), A(u)
        &\vdash
        \exists xA(x)\rightarrow\forall x B(x) &(\in)\\
        \exists xA(x)\rightarrow\forall x B(x), A(u)
        &\vdash
        \forall xB(x) &(\rightarrow^-)\\
        \exists xA(x)\rightarrow\forall x B(x), A(u)
        &\vdash
        B(u) &(\forall^-)\\
        \exists xA(x)\rightarrow\forall x B(x)
        &\vdash
        A(u)\rightarrow B(u) &(\rightarrow^+)\\
        \exists xA(x)\rightarrow\forall x B(x)
        &\vdash
        \forall x(A(x)\rightarrow B(x)) &(\forall^-)\\
        &\vdash
        (\exists xA(x)\rightarrow\forall x B(x))
        \rightarrow
        \forall x(A(x)\rightarrow B(x)) &(\rightarrow^+)
    \end{align*}
\end{solution}
\begin{problem}
\begin{equation*}
    \vdash
    \exists y(r(y)\rightarrow\forall y r(y)),
\end{equation*}
where $r$ is a unary predicate symbol.
\end{problem}
\begin{solution}
    \begin{align*}
        \exists y(r(y)\rightarrow\forall y r(y))
        &\vdash \forall y\neg(r(y)\rightarrow\forall y r(y))&(\text{1.1题结论})\\
        \exists y(r(y)\rightarrow\forall y r(y))
        &\vdash \neg(r(u)\rightarrow\forall y r(y))&(\forall^-)\\
        \neg(r(u)\rightarrow\forall y r(y))
        &\vdash r(u)\land\neg\forall yr(y)&(\text{引理2})\\
        \exists y(r(y)\rightarrow\forall y r(y))
        &\vdash r(u)\land\neg\forall yr(y)&(\text{trans})\\
        \exists y(r(y)\rightarrow\forall y r(y))
        &\vdash r(u) &(\land^-)\\
        \exists y(r(y)\rightarrow\forall y r(y))
        &\vdash \neg\forall yr(y)&(\land^-)\\
        \exists y(r(y)\rightarrow\forall y r(y))
        &\vdash \forall yr(y) &(\forall^+)\\
        &\vdash
        \exists y(r(y)\rightarrow\forall y r(y)) &(\neg^-)
    \end{align*}
\end{solution}
\end{document}